Source/DafnyStandardLibraries/src/DafnyStdLibs/DisableNonLinearArithmetic/Strings.dfy
@@ -7,21 +7,28 @@ module DafnyStdLibs.Strings {
   import opened Arithmetic.Logarithm
   import Arithmetic
 
+  /**
+  Refine this module to use it.
+  The refinee must define:
+    - the type of character used, Char
+    - a conversion from nat to Char and vice versa
+   */
   abstract module ParametricConversion refines Arithmetic.LittleEndianNat {
     import opened Wrappers
 
     type Char(==)
     type String = seq<Char>
-    type CharSet = chars: seq<Char> | |chars| > 1 witness *
-    const chars: CharSet
+
+    type CharSeq = chars: seq<Char> | |chars| > 1 witness *
+    const chars: CharSeq
     const base := |chars|
-    const charMap: map<Char, uint>
+    const charToDigit: map<Char, digit>
 
     function BASE(): nat {
       base
     }
 
-    function OfDigits(digits: seq<uint>) : (str: String)
+    function OfDigits(digits: seq<digit>) : (str: String)
       requires forall d | d in digits :: 0 <= d < base
       ensures forall c <- str :: c in chars
       ensures |str| == |digits|
@@ -33,6 +40,9 @@ module DafnyStdLibs.Strings {
         OfDigits(digits[1..]) + [chars[digits[0]]]
     }
 
+    /*
+    Convert a natural number into its String representation
+    */
     function OfNat(n: nat) : (str: String)
       ensures |str| == Log(base, n) + 1
       ensures forall c <- str :: c in chars
@@ -49,10 +59,14 @@ module DafnyStdLibs.Strings {
 
     predicate ToNumberStr(str: String, minus: Char) {
       str != [] ==>
-        && (str[0] == minus || str[0] in charMap)
-        && forall c <- str[1..] :: c in charMap
+        && (str[0] == minus || str[0] in charToDigit)
+        && forall c <- str[1..] :: c in charToDigit
     }
 
+    /*
+    Convert an integer into its String representation, 
+    given a particular minus character.
+    */
     function OfInt(n: int, minus: Char) : (str: String)
       ensures OfNumberStr(str, minus)
     {
@@ -60,19 +74,22 @@ module DafnyStdLibs.Strings {
       else [minus] + OfNat(-n)
     }
 
+    /**
+    Convert a String that represents a natural number, back into that number.
+     */
     function {:vcs_split_on_every_assert} ToNat(str: String) : (n: nat)
-      requires forall c <- str :: c in charMap
+      requires forall c <- str :: c in charToDigit
     {
       if str == [] then 0
       else
         LemmaMulNonnegativeAuto();
-        ToNat(str[..|str| - 1]) * base + charMap[str[|str| - 1]]
+        ToNat(str[..|str| - 1]) * base + charToDigit[str[|str| - 1]]
     }
 
     lemma {:induction false} ToNatBound(str: String)
       requires base > 0
-      requires forall c <- str :: c in charMap
-      requires forall c <- str :: charMap[c] < base
+      requires forall c <- str :: c in charToDigit
+      requires forall c <- str :: charToDigit[c] < base
       ensures ToNat(str) < Pow(base, |str|)
     {
       if str == [] {
@@ -80,7 +97,7 @@ module DafnyStdLibs.Strings {
       } else {
         calc <= {
           ToNat(str);
-          ToNat(str[..|str| - 1]) * base + charMap[str[|str| - 1]];
+          ToNat(str[..|str| - 1]) * base + charToDigit[str[|str| - 1]];
           ToNat(str[..|str| - 1]) * base + (base - 1);
           { ToNatBound(str[..|str| - 1]);
             LemmaMulInequalityAuto(); }
@@ -93,6 +110,9 @@ module DafnyStdLibs.Strings {
       }
     }
 
+    /**
+    Convert a String that represents a number, back into that number
+     */
     function ToInt(str: String, minus: Char): (s: int)
       requires str != [minus]
       requires ToNumberStr(str, minus)
@@ -110,26 +130,29 @@ module DafnyStdLibs.Strings {
     type Char(==)
     type String = seq<Char>
 
-    function Escape(str: String, special: set<Char>, escape: Char): String {
+    /**
+    Use an escape character to convert a String to its escaped form.
+     */
+    function Escape(str: String, mustEscape: set<Char>, escape: Char): String {
       if str == [] then str
-      else if str[0] in special then [escape, str[0]] + Escape(str[1..], special, escape)
-      else [str[0]] + Escape(str[1..], special, escape)
+      else if str[0] in mustEscape then [escape, str[0]] + Escape(str[1..], mustEscape, escape)
+      else [str[0]] + Escape(str[1..], mustEscape, escape)
     }
 
-    datatype UnescapeError =
-      EscapeAtEOS
-
-    function Unescape(str: String, escape: Char): Result<String, UnescapeError> {
-      if str == [] then Success(str)
+    /**
+    Unescape a String using the given escape character.
+     */
+    function Unescape(str: String, escape: Char): Option<String> {
+      if str == [] then Some(str)
       else if str[0] == escape then
-        if |str| > 1 then var tl :- Unescape(str[2..], escape); Success([str[1]] + tl)
-        else Failure(EscapeAtEOS)
-      else var tl :- Unescape(str[1..], escape); Success([str[0]] + tl)
+        if |str| > 1 then var tl :- Unescape(str[2..], escape); Some([str[1]] + tl)
+        else None
+      else var tl :- Unescape(str[1..], escape); Some([str[0]] + tl)
     }
 
     lemma {:induction false} Unescape_Escape(str: String, special: set<Char>, escape: Char)
       requires escape in special
-      ensures Unescape(Escape(str, special, escape), escape) == Success(str)
+      ensures Unescape(Escape(str, special, escape), escape) == Some(str)
     {
       if str == [] {
       } else {
@@ -143,7 +166,7 @@ module DafnyStdLibs.Strings {
     type Char = char
     const HEX_DIGITS: seq<char> := "0123456789ABCDEF"
     const chars := HEX_DIGITS
-    const charMap :=
+    const charToDigit :=
       map[
         '0' := 0, '1' := 1, '2' := 2, '3' := 3, '4' := 4, '5' := 5, '6' := 6, '7' := 7, '8' := 8, '9' := 9,
         'a' := 0xA, 'b' := 0xB, 'c' := 0xC, 'd' := 0xD, 'e' := 0xE, 'f' := 0xF,
@@ -155,7 +178,7 @@ module DafnyStdLibs.Strings {
     type Char = char
     const DIGITS: seq<char> := "0123456789"
     const chars := DIGITS
-    const charMap :=
+    const charToDigit :=
       map[
         '0' := 0, '1' := 1, '2' := 2, '3' := 3, '4' := 4, '5' := 5, '6' := 6, '7' := 7, '8' := 8, '9' := 9
       ]
@@ -165,6 +188,9 @@ module DafnyStdLibs.Strings {
     type Char = char
   }
 
+  /*
+  Convert a natural number into its String representation for a decimal number system
+  */
   function OfNat(n: nat) : (str: string)
     ensures |str| == Log(DecimalConversion.base, n) + 1
     ensures forall c | c in str :: c in DecimalConversion.chars
@@ -172,20 +198,29 @@ module DafnyStdLibs.Strings {
     DecimalConversion.OfNat(n)
   }
 
+  /*
+  Convert an integer into its String representation for a decimal number system
+  */
   function OfInt(n: int) : (str: string)
     ensures DecimalConversion.OfNumberStr(str, '-')
   {
     DecimalConversion.OfInt(n, '-')
   }
 
+  /**
+  Given a natural number represented as a decimal number in a String, back into an integer
+   */
   function ToNat(str: string) : (n: nat)
-    requires forall c <- str :: c in DecimalConversion.charMap && DecimalConversion.charMap[c] as int < DecimalConversion.base
+    requires forall c <- str :: c in DecimalConversion.charToDigit && DecimalConversion.charToDigit[c] as int < DecimalConversion.base
     ensures n < Pow(DecimalConversion.base, |str|)
   {
     DecimalConversion.ToNatBound(str);
     DecimalConversion.ToNat(str)
   }
 
+  /**
+  Given an integer number represented as a decimal number in a String, back into an integer
+   */
   function ToInt(str: string) : (n: int)
     requires str != "-"
     requires DecimalConversion.ToNumberStr(str, '-')
@@ -193,29 +228,46 @@ module DafnyStdLibs.Strings {
     DecimalConversion.ToInt(str, '-')
   }
 
+  /**
+  Use an escape character to convert a String to its escaped form.
+    */
   function EscapeQuotes(str: string): string {
     CharStrEscaping.Escape(str, {'\"', '\''}, '\\')
   }
 
-  function UnescapeQuotes(str: string): Result<string, CharStrEscaping.UnescapeError> {
+  /**
+  Unescape a String using the given escape character.
+    */
+  function UnescapeQuotes(str: string): Option<string> {
     CharStrEscaping.Unescape(str, '\\')
   }
 
-
+  /**
+  Convert a boolean into its string representation
+   */
   function OfBool(b: bool) : string {
     if b then "true" else "false"
   }
 
+  /**
+  Convert a char into its string representation
+   */
   function OfChar(c: char) : string {
     [c]
   }
 
+  /**
+  Join a sequence of strings using a separator string
+   */
   function Join(sep: string, strs: seq<string>) : string {
     if |strs| == 0 then ""
     else if |strs| == 1 then strs[0]
     else strs[0] + sep + Join(sep, strs[1..])
   }
 
+  /**
+  Concatenate a sequence of strings
+   */
   function Concat(strs: seq<string>) : string {
     if |strs| == 0 then ""
     else strs[0] + Concat(strs[1..])
